language_formal/spark2014_semantics/spark2014_core_subset(non-nested)/semantics.v
@@ -50,7 +50,7 @@ Inductive do_division_check: binary_operator -> value -> value -> check_status -
         do_division_check Divide (BasicV (Int v1)) (BasicV (Int v2)) (Exception RTE_Division_By_Zero).
 
 Inductive do_range_check: Z -> Z -> Z -> check_status -> Prop :=
-    | Do_Range_Check: forall i l u,
+    | Do_Range_Check_OK: forall i l u,
         (* i >= l /\ u >= i *)
         (Zge_bool i l) && (Zge_bool u i) = true ->
         do_range_check i l u Success
@@ -181,19 +181,39 @@ with eval_name: symboltable -> stack -> name -> Return value -> Prop :=
     | Eval_E_Identifier: forall x s v st ast_num, 
         fetchG x s = Some v ->
         eval_name st s (E_Identifier ast_num x) (Normal v)
-    | Eval_E_Indexed_Component_RTE_E: forall st s e msg ast_num x_ast_num x,
+    | Eval_E_Indexed_Component_RTE: forall st s e msg ast_num x_ast_num x,
         eval_expr st s e (Run_Time_Error msg) ->
         eval_name st s (E_Indexed_Component ast_num x_ast_num x e) (Run_Time_Error msg)
-    | Eval_E_Indexed_Component_RTE_Index: forall st s e i x_ast_num t a_ast_num tn typ l u ast_num x, 
+    | Eval_E_Indexed_Component_SubtypeMark_RTE: forall st s e i x_ast_num tn a_ast_num tm typ tn' t l u ast_num x, 
         eval_expr st s e (Normal (BasicV (Int i))) ->
-        fetch_exp_type x_ast_num st = Some (Array_Type t) ->
-        fetch_type t st = Some (Array_Type_Declaration a_ast_num tn typ l u) ->
+        fetch_exp_type x_ast_num st = Some (Array_Type tn) ->
+        fetch_type tn st = Some (Array_Type_Declaration_SubtypeMark a_ast_num tn tm typ) ->
+        subtype_num tm = Some tn' ->
+        fetch_type tn' st = Some t ->
+        subtype_range t = Some (Range l u) ->
         do_range_check i l u (Exception RTE_Range) ->
         eval_name st s (E_Indexed_Component ast_num x_ast_num x e) (Run_Time_Error RTE_Range)
-    | Eval_E_Indexed_Component: forall st s e i x_ast_num t a_ast_num tn typ l u x a v ast_num, 
+    | Eval_E_Indexed_Component_Range_RTE: forall st s e i x_ast_num t a_ast_num l u typ ast_num x, 
         eval_expr st s e (Normal (BasicV (Int i))) ->
         fetch_exp_type x_ast_num st = Some (Array_Type t) ->
-        fetch_type t st = Some (Array_Type_Declaration a_ast_num tn typ l u) ->        
+        fetch_type t st = Some (Array_Type_Declaration_Range a_ast_num t (Range l u) typ) ->
+        do_range_check i l u (Exception RTE_Range) ->
+        eval_name st s (E_Indexed_Component ast_num x_ast_num x e) (Run_Time_Error RTE_Range)
+    | Eval_E_Indexed_Component_SubtypeMark: forall st s e i x_ast_num tn a_ast_num tm typ tn' t l u x a v ast_num, 
+        eval_expr st s e (Normal (BasicV (Int i))) ->
+        fetch_exp_type x_ast_num st = Some (Array_Type tn) ->
+        fetch_type tn st = Some (Array_Type_Declaration_SubtypeMark a_ast_num tn tm typ) ->
+        subtype_num tm = Some tn' ->
+        fetch_type tn' st = Some t ->
+        subtype_range t = Some (Range l u) ->
+        do_range_check i l u Success ->
+        fetchG x s = Some (AggregateV (ArrayV a)) ->
+        array_select a i = Some v ->
+        eval_name st s (E_Indexed_Component ast_num x_ast_num x e) (Normal (BasicV v))
+    | Eval_E_Indexed_Component_Range: forall st s e i x_ast_num t a_ast_num l u typ x a v ast_num, 
+        eval_expr st s e (Normal (BasicV (Int i))) ->
+        fetch_exp_type x_ast_num st = Some (Array_Type t) ->
+        fetch_type t st = Some (Array_Type_Declaration_Range a_ast_num t (Range l u) typ) ->        
         do_range_check i l u Success ->
         fetchG x s = Some (AggregateV (ArrayV a)) ->
         array_select a i = Some v ->
@@ -202,6 +222,7 @@ with eval_name: symboltable -> stack -> name -> Return value -> Prop :=
         fetchG x s = Some (AggregateV (RecordV r)) ->
         record_select r f = Some v ->
         eval_name st s (E_Selected_Component ast_num x_ast_num x f) (Normal (BasicV v)).
+
 
 (** ** Statement Evaluation Semantics *)
 
@@ -223,19 +244,43 @@ with eval_name: symboltable -> stack -> name -> Return value -> Prop :=
   - [s'] is the resulting state. *)
 
 (** *** Copy Out *)
-Inductive copy_out: stack -> frame -> list parameter_specification -> list expression -> stack -> Prop :=
-    | Copy_Out_Nil : forall s f, 
-        copy_out s f nil nil s
-    | Copy_Out_Cons_Out: forall s s' s'' v f param lparam lexp x ast_num x_ast_num,
+Inductive copy_out: symboltable -> stack -> frame -> list parameter_specification -> list expression -> Return stack -> Prop :=
+    | Copy_Out_Nil : forall st s f, 
+        copy_out st s f nil nil (Normal s)
+    | Copy_Out_Cons_Out: forall st s s' s'' t v f param lparam lexp x ast_num x_ast_num,
         param.(parameter_mode) = Out ->
+        fetch_exp_type ast_num st = Some t ->
+        is_range_constrainted_type t = false ->
         fetch param.(parameter_name) f = Some v ->
         updateG s x v = Some s' ->
-        copy_out s' f lparam lexp s'' ->
-        copy_out s f (param :: lparam) ((E_Name ast_num (E_Identifier x_ast_num x)) :: lexp) s''
-    | Copy_Out_Cons_In: forall s s' f param lparam lexp e,
+        copy_out st s' f lparam lexp s'' ->
+        copy_out st s f (param :: lparam) ((E_Name ast_num (E_Identifier x_ast_num x)) :: lexp) s''
+    | Copy_Out_Cons_Out_Range_RTE: forall st t tn td l u f v s param lparam lexp x ast_num x_ast_num,
+        param.(parameter_mode) = Out ->
+        fetch_exp_type ast_num st = Some t ->
+        is_range_constrainted_type t = true ->
+        subtype_num t = Some tn ->
+        fetch_type tn st = Some td ->
+        subtype_range td = Some (Range l u) ->
+        fetch param.(parameter_name) f = Some (BasicV (Int v)) ->
+        do_range_check v l u (Exception RTE_Range) ->
+        copy_out st s f (param :: lparam) ((E_Name ast_num (E_Identifier x_ast_num x)) :: lexp) (Run_Time_Error RTE_Range)
+    | Copy_Out_Cons_Out_Range: forall st t tn td l u f v s s' s'' param lparam lexp x ast_num x_ast_num,
+        param.(parameter_mode) = Out ->
+        fetch_exp_type ast_num st = Some t ->
+        is_range_constrainted_type t = true ->
+        subtype_num t = Some tn ->
+        fetch_type tn st = Some td ->
+        subtype_range td = Some (Range l u) ->
+        fetch param.(parameter_name) f = Some (BasicV (Int v)) ->
+        do_range_check v l u Success ->
+        updateG s x (BasicV (Int v)) = Some s' ->
+        copy_out st s' f lparam lexp s'' ->
+        copy_out st s f (param :: lparam) ((E_Name ast_num (E_Identifier x_ast_num x)) :: lexp) s''
+    | Copy_Out_Cons_In: forall st s s' f param lparam lexp e,
         param.(parameter_mode) = In ->
-        copy_out s f lparam lexp s' ->
-        copy_out s f (param :: lparam) (e :: lexp) s'.
+        copy_out st s f lparam lexp s' ->
+        copy_out st s f (param :: lparam) (e :: lexp) s'.
 
 (** [Copy_in s lparams lexp frame] means the frame is the portion of
     stack to push on the stack to start evaluating the procedure
@@ -248,31 +293,57 @@ Inductive copy_out: stack -> frame -> list parameter_specification -> list expre
 (* start from an empty frame and then push the values of arguments into it *)
 
 (** *** Copy In *)
-Inductive copy_in: stack -> frame -> list parameter_specification -> list expression -> Return frame -> Prop :=
-    | Copy_In_Nil : forall s f, 
-        copy_in s f nil nil (Normal f)
-    | Copy_In_Cons_Out: forall param s f lparam le f' ast_num x_ast_num x,
+Inductive copy_in: symboltable -> stack -> frame -> list parameter_specification -> list expression -> Return frame -> Prop :=
+    | Copy_In_Nil : forall st s f, 
+        copy_in st s f nil nil (Normal f)
+    | Copy_In_Cons_Out_RTE: forall param st s f lparam le msg ast_num x_ast_num x,
         param.(parameter_mode) = Out ->
-        copy_in s f lparam le (Normal f') ->
-        copy_in s f (param :: lparam) ((E_Name ast_num (E_Identifier x_ast_num x)) :: le) (Normal (push f' param.(parameter_name) Undefined))
-    | Copy_In_Cons_Out_E: forall param s f lparam le msg ast_num x_ast_num x,
+        copy_in st s f lparam le (Run_Time_Error msg) ->
+        copy_in st s f (param :: lparam) (E_Name ast_num (E_Identifier x_ast_num x) :: le) (Run_Time_Error msg)
+    | Copy_In_Cons_Out: forall param st s f lparam le f' ast_num x_ast_num x,
         param.(parameter_mode) = Out ->
-        copy_in s f lparam le (Run_Time_Error msg) ->
-        copy_in s f (param :: lparam) (E_Name ast_num (E_Identifier x_ast_num x) :: le) (Run_Time_Error msg)
-    | Copy_In_Cons_In: forall param s e v f lparam le f',
+        copy_in st s f lparam le (Normal f') ->
+        copy_in st s f (param :: lparam) ((E_Name ast_num (E_Identifier x_ast_num x)) :: le) (Normal (push f' param.(parameter_name) Undefined))
+    | Copy_In_Cons_In_RTE: forall param st s e msg f lparam le,
         param.(parameter_mode) = In ->
-        eval_expr s e (Normal v) ->
-        copy_in s f lparam le (Normal f') ->
-        copy_in s f (param :: lparam) (e :: le) (Normal (push f' param.(parameter_name) v))
-    | Copy_In_Cons_In_E1: forall param s e msg f lparam le,
+        eval_expr st s e (Run_Time_Error msg) ->
+        copy_in st s f (param :: lparam) (e :: le) (Run_Time_Error msg)
+    | Copy_In_Cons_In: forall param st s e v f lparam le f',
         param.(parameter_mode) = In ->
-        eval_expr s e (Run_Time_Error msg) ->
-        copy_in s f (param :: lparam) (e :: le) (Run_Time_Error msg)
-    | Copy_In_Cons_In_E2: forall param s e v f lparam le msg,
+        eval_expr st s e (Normal v) ->
+        is_range_constrainted_type (param.(parameter_subtype_mark)) = false ->
+        copy_in st s f lparam le (Normal f') ->
+        copy_in st s f (param :: lparam) (e :: le) (Normal (push f' param.(parameter_name) v))
+    | Copy_In_Cons_In_Range_RTE: forall param st s e v tn td l u f lparam le,
         param.(parameter_mode) = In ->
-        eval_expr s e (Normal v) ->
-        copy_in s f lparam le (Run_Time_Error msg) ->
-        copy_in s f (param :: lparam) (e :: le) (Run_Time_Error msg).
+        eval_expr st s e (Normal (BasicV (Int v))) ->
+        is_range_constrainted_type (param.(parameter_subtype_mark)) = true ->
+        subtype_num (param.(parameter_subtype_mark)) = Some tn ->
+        fetch_type tn st = Some td ->
+        subtype_range td = Some (Range l u) ->
+        do_range_check v l u (Exception RTE_Range) ->
+        copy_in st s f (param :: lparam) (e :: le) (Run_Time_Error RTE_Range)
+    | Copy_In_Cons_In_Range_RTE_Tail: forall param st s e v tn td l u f msg lparam le,
+        param.(parameter_mode) = In ->
+        eval_expr st s e (Normal (BasicV (Int v))) ->
+        is_range_constrainted_type (param.(parameter_subtype_mark)) = true ->
+        subtype_num (param.(parameter_subtype_mark)) = Some tn ->
+        fetch_type tn st = Some td ->
+        subtype_range td = Some (Range l u) ->
+        do_range_check v l u Success ->
+        copy_in st s f lparam le (Run_Time_Error msg) ->
+        copy_in st s f (param :: lparam) (e :: le) (Run_Time_Error msg)
+    | Copy_In_Cons_In_Range: forall param st s e v tn td l u f f' lparam le,
+        param.(parameter_mode) = In ->
+        eval_expr st s e (Normal (BasicV (Int v))) ->
+        is_range_constrainted_type (param.(parameter_subtype_mark)) = true ->
+        subtype_num (param.(parameter_subtype_mark)) = Some tn ->
+        fetch_type tn st = Some td ->
+        subtype_range td = Some (Range l u) ->
+        do_range_check v l u Success ->
+        copy_in st s f lparam le (Normal f') ->
+        copy_in st s f (param :: lparam) (e :: le) (Normal (push f' param.(parameter_name) (BasicV (Int v)))).
+
 
 (** ** Declaration Evaluation Semantics *)
 (** Inductive semantic of declarations. [eval_decl s nil decl
@@ -281,36 +352,51 @@ Inductive copy_in: stack -> frame -> list parameter_specification -> list expres
     the frame.
  *)
 
-Inductive eval_decl: stack -> frame -> declaration -> Return frame -> Prop :=
-    | Eval_Decl_Null: forall s f,
-        eval_decl s f D_Null_Declaration (Normal f)
-    | Eval_Decl_Type: forall s f ast_num t,
-        eval_decl s f (D_Type_Declaration ast_num t) (Normal f)
-    | Eval_Decl_E: forall d e f s msg ast_num,
-        d.(initialization_expression) = Some e ->
-        eval_expr (f :: s) e (Run_Time_Error msg) ->
-        eval_decl s f (D_Object_Declaration ast_num d) (Run_Time_Error msg)
-    | Eval_Decl: forall d e f s v ast_num,
-        d.(initialization_expression) = Some e ->
-        eval_expr (f :: s) e (Normal v) ->
-        eval_decl s f (D_Object_Declaration ast_num d) (Normal (push f d.(object_name) v))
-    | Eval_UndefDecl: forall d s f ast_num,
+Inductive eval_decl: symboltable -> stack -> frame -> declaration -> Return frame -> Prop :=
+    | Eval_Decl_Null: forall st s f,
+        eval_decl st s f D_Null_Declaration (Normal f)
+    | Eval_Decl_Type: forall st s f ast_num t,
+        eval_decl st s f (D_Type_Declaration ast_num t) (Normal f)
+    | Eval_Decl_Var_None: forall d st s f ast_num,
         d.(initialization_expression) = None ->
-        eval_decl s f (D_Object_Declaration ast_num d) (Normal (push f d.(object_name) Undefined))
-    | Eval_Decl_Proc: forall s f ast_num p,
-        eval_decl s f (D_Procedure_Body ast_num p) (Normal f)
-    | Eval_Decl_Seq_E: forall s f d1 msg ast_num d2,
-        eval_decl s f d1 (Run_Time_Error msg) ->
-        eval_decl s f (D_Seq_Declaration ast_num d1 d2) (Run_Time_Error msg)
-    | Eval_Decl_Seq: forall s f d1 f' d2 f'' ast_num,
-        eval_decl s f d1 (Normal f') ->
-        eval_decl s f d2 f'' ->
-        eval_decl s f (D_Seq_Declaration ast_num d1 d2) f''.
-(*  | Eval_Decl_Proc: forall s f ast_num p,
-        eval_decl s f (D_Procedure_Declaration ast_num p) (Normal (push f (procedure_name p) (Procedure p)))
-    | Eval_Decl_Type: forall s f ast_num t,
-        eval_decl s f (D_Type_Declaration ast_num t) (Normal (push frm (type_name t) (TypeDef t)))
-*)
+        eval_decl st s f (D_Object_Declaration ast_num d) (Normal (push f d.(object_name) Undefined))
+    | Eval_Decl_Var_RTE: forall d e st f s msg ast_num,
+        d.(initialization_expression) = Some e ->
+        eval_expr st (f :: s) e (Run_Time_Error msg) ->
+        eval_decl st s f (D_Object_Declaration ast_num d) (Run_Time_Error msg)
+    | Eval_Decl_Var: forall d e st f s v ast_num,
+        d.(initialization_expression) = Some e ->
+        eval_expr st (f :: s) e (Normal v) ->
+        is_range_constrainted_type (d.(object_nominal_subtype)) = false ->
+        eval_decl st s f (D_Object_Declaration ast_num d) (Normal (push f d.(object_name) v))
+    | Eval_Decl_Var_Range_RTE: forall d e st f s v tn td l u ast_num,
+        d.(initialization_expression) = Some e ->
+        eval_expr st (f :: s) e (Normal (BasicV (Int v))) ->
+        is_range_constrainted_type (d.(object_nominal_subtype)) = true ->
+        subtype_num (d.(object_nominal_subtype)) = Some tn ->
+        fetch_type tn st = Some td ->
+        subtype_range td = Some (Range l u) ->
+        do_range_check v l u (Exception RTE_Range) ->        
+        eval_decl st s f (D_Object_Declaration ast_num d) (Run_Time_Error RTE_Range)
+    | Eval_Decl_Var_Range: forall d e st f s v tn td l u ast_num,
+        d.(initialization_expression) = Some e ->
+        eval_expr st (f :: s) e (Normal (BasicV (Int v))) ->
+        is_range_constrainted_type (d.(object_nominal_subtype)) = true ->
+        subtype_num (d.(object_nominal_subtype)) = Some tn ->
+        fetch_type tn st = Some td ->
+        subtype_range td = Some (Range l u) ->
+        do_range_check v l u Success ->        
+        eval_decl st s f (D_Object_Declaration ast_num d) (Normal (push f d.(object_name) (BasicV (Int v))))
+    | Eval_Decl_Proc: forall st s f ast_num p,
+        eval_decl st s f (D_Procedure_Body ast_num p) (Normal f)
+    | Eval_Decl_Seq_RTE: forall st s f d1 msg ast_num d2,
+        eval_decl st s f d1 (Run_Time_Error msg) ->
+        eval_decl st s f (D_Seq_Declaration ast_num d1 d2) (Run_Time_Error msg)
+    | Eval_Decl_Seq: forall st s f d1 f' d2 f'' ast_num,
+        eval_decl st s f d1 (Normal f') ->
+        eval_decl st s f d2 f'' ->
+        eval_decl st s f (D_Seq_Declaration ast_num d1 d2) f''.
+
 
 (* a[i] := v *)
 Function arrayUpdate (a: list (index * basic_value)) (i: index) (v: basic_value): list (index * basic_value) :=
@@ -369,66 +455,87 @@ Qed.
 Inductive eval_stmt: symboltable -> stack -> statement -> Return stack -> Prop := 
     | Eval_S_Null: forall st s,
         eval_stmt st s S_Null (Normal s)
-    | Eval_S_Assignment_RTE: forall s e msg st ast_num x,
-        eval_expr s e (Run_Time_Error msg) ->
+    | Eval_S_Assignment_RTE: forall st s e msg ast_num x,
+        eval_expr st s e (Run_Time_Error msg) ->
         eval_stmt st s (S_Assignment ast_num x e) (Run_Time_Error msg)
-    | Eval_S_Assignment: forall s e v x s1 st ast_num,
-        eval_expr s e (Normal v) ->
-        storeUpdate s x v s1 ->
+    | Eval_S_Assignment: forall st s e v x t s1 ast_num,
+        eval_expr st s e (Normal v) ->
+        fetch_exp_type (name_astnum x) st = Some t ->
+        is_range_constrainted_type t = false ->
+        storeUpdate st s x v s1 ->
         eval_stmt st s (S_Assignment ast_num x e) s1
-    | Eval_S_If_RTE: forall s b msg st ast_num c1 c2,
-        eval_expr s b (Run_Time_Error msg) ->
+    | Eval_S_Assignment_Range_RTE: forall st s e v x t tn td l u ast_num,
+        eval_expr st s e (Normal (BasicV (Int v))) ->
+        fetch_exp_type (name_astnum x) st = Some t ->
+        is_range_constrainted_type t = true ->
+        subtype_num t = Some tn ->
+        fetch_type tn st = Some td ->
+        subtype_range td = Some (Range l u) ->
+        do_range_check v l u (Exception RTE_Range) ->
+        eval_stmt st s (S_Assignment ast_num x e) (Run_Time_Error RTE_Range)
+    | Eval_S_Assignment_Range: forall st s e v x t tn td l u s1 ast_num,
+        eval_expr st s e (Normal (BasicV (Int v))) ->
+        fetch_exp_type (name_astnum x) st = Some t ->
+        is_range_constrainted_type t = true ->
+        subtype_num t = Some tn ->
+        fetch_type tn st = Some td ->
+        subtype_range td = Some (Range l u) ->
+        do_range_check v l u Success ->
+        storeUpdate st s x (BasicV (Int v)) s1 ->
+        eval_stmt st s (S_Assignment ast_num x e) s1
+    | Eval_S_If_RTE: forall st s b msg ast_num c1 c2,
+        eval_expr st s b (Run_Time_Error msg) ->
         eval_stmt st s (S_If ast_num b c1 c2) (Run_Time_Error msg)
-    | Eval_S_If_True: forall s b st c1 s1 ast_num c2,
-        eval_expr s b (Normal (BasicV (Bool true))) ->
+    | Eval_S_If_True: forall st s b c1 s1 ast_num c2,
+        eval_expr st s b (Normal (BasicV (Bool true))) ->
         eval_stmt st s c1 s1 ->
         eval_stmt st s (S_If ast_num b c1 c2) s1
-    | Eval_S_If_False: forall s b st c2 s1 ast_num c1,
-        eval_expr s b (Normal (BasicV (Bool false))) ->
+    | Eval_S_If_False: forall st s b c2 s1 ast_num c1,
+        eval_expr st s b (Normal (BasicV (Bool false))) ->
         eval_stmt st s c2 s1 ->
         eval_stmt st s (S_If ast_num b c1 c2) s1
-    | Eval_S_While_Loop_RTE: forall s b msg st ast_num c,
-        eval_expr s b (Run_Time_Error msg) ->
+    | Eval_S_While_Loop_RTE: forall st s b msg ast_num c,
+        eval_expr st s b (Run_Time_Error msg) ->
         eval_stmt st s (S_While_Loop ast_num b c) (Run_Time_Error msg)
-    | Eval_S_While_Loop_True_RTE: forall s b st c msg ast_num,
-        eval_expr s b (Normal (BasicV (Bool true))) ->
+    | Eval_S_While_Loop_True_RTE: forall st s b c msg ast_num,
+        eval_expr st s b (Normal (BasicV (Bool true))) ->
         eval_stmt st s c (Run_Time_Error msg) ->
         eval_stmt st s (S_While_Loop ast_num b c) (Run_Time_Error msg)
-    | Eval_S_While_Loop_True: forall s b st c s1 ast_num s2,
-        eval_expr s b (Normal (BasicV (Bool true))) ->
+    | Eval_S_While_Loop_True: forall st s b c s1 ast_num s2,
+        eval_expr st s b (Normal (BasicV (Bool true))) ->
         eval_stmt st s c (Normal s1) ->
         eval_stmt st s1 (S_While_Loop ast_num b c) s2 ->
         eval_stmt st s (S_While_Loop ast_num b c) s2
-    | Eval_S_While_Loop_False: forall s b st ast_num c,
-        eval_expr s b (Normal (BasicV (Bool false))) ->
+    | Eval_S_While_Loop_False: forall st s b ast_num c,
+        eval_expr st s b (Normal (BasicV (Bool false))) ->
         eval_stmt st s (S_While_Loop ast_num b c) (Normal s)
     | Eval_S_Proc_RTE_Args: forall p st n pb s args msg ast_num p_ast_num,
         fetch_proc p st = Some (n, pb) ->
-        copy_in s (newFrame n) (procedure_parameter_profile pb) args (Run_Time_Error msg) ->
+        copy_in st s (newFrame n) (procedure_parameter_profile pb) args (Run_Time_Error msg) ->
         eval_stmt st s (S_Procedure_Call ast_num p_ast_num p args) (Run_Time_Error msg)
     | Eval_S_Proc_RTE_Decl: forall p st n pb s args f intact_s s1 msg ast_num p_ast_num,
         fetch_proc p st = Some (n, pb) ->
-        copy_in s (newFrame n) (procedure_parameter_profile pb) args (Normal f) ->
+        copy_in st s (newFrame n) (procedure_parameter_profile pb) args (Normal f) ->
         cut_until s n intact_s s1 -> (* s = intact_s ++ s1 *)
-        eval_decl s1 f (procedure_declarative_part pb) (Run_Time_Error msg) ->
+        eval_decl st s1 f (procedure_declarative_part pb) (Run_Time_Error msg) ->
         eval_stmt st s (S_Procedure_Call ast_num p_ast_num p args) (Run_Time_Error msg)
     | Eval_S_Proc_RTE_Body: forall p st n pb s args f intact_s s1 f1 msg ast_num p_ast_num,
         fetch_proc p st = Some (n, pb) ->
-        copy_in s (newFrame n) (procedure_parameter_profile pb) args (Normal f) ->
+        copy_in st s (newFrame n) (procedure_parameter_profile pb) args (Normal f) ->
         cut_until s n intact_s s1 -> (* s = intact_s ++ s1 *)
-        eval_decl s1 f (procedure_declarative_part pb) (Normal f1) ->
+        eval_decl st s1 f (procedure_declarative_part pb) (Normal f1) ->
         eval_stmt st (f1 :: s1) (procedure_statements pb) (Run_Time_Error msg) ->
         eval_stmt st s (S_Procedure_Call ast_num p_ast_num p args) (Run_Time_Error msg)
     | Eval_S_Proc: forall p st n pb s args f intact_s s1 f1 s2 locals_section params_section s3 s4 ast_num p_ast_num,
         fetch_proc p st = Some (n, pb) ->
-        copy_in s (newFrame n) (procedure_parameter_profile pb) args (Normal f) ->
+        copy_in st s (newFrame n) (procedure_parameter_profile pb) args (Normal f) ->
         cut_until s n intact_s s1 -> (* s = intact_s ++ s1 *)
-        eval_decl s1 f (procedure_declarative_part pb) (Normal f1) ->          
+        eval_decl st s1 f (procedure_declarative_part pb) (Normal f1) ->          
         eval_stmt st (f1 :: s1) (procedure_statements pb) (Normal s2) ->
         s2 = (n, locals_section ++ params_section) :: s3 -> (* extract parameters from local frame *)
         length (store_of f) = length params_section ->
-        copy_out (intact_s ++ s3) (n, params_section) (procedure_parameter_profile pb) args s4 ->
-        eval_stmt st s (S_Procedure_Call ast_num p_ast_num p args) (Normal s4)
+        copy_out st (intact_s ++ s3) (n, params_section) (procedure_parameter_profile pb) args s4 ->
+        eval_stmt st s (S_Procedure_Call ast_num p_ast_num p args) s4
     | Eval_S_Sequence_RTE: forall st s c1 msg ast_num c2,
         eval_stmt st s c1 (Run_Time_Error msg) ->
         eval_stmt st s (S_Sequence ast_num c1 c2) (Run_Time_Error msg)
@@ -437,31 +544,80 @@ Inductive eval_stmt: symboltable -> stack -> statement -> Return stack -> Prop :
         eval_stmt st s1 c2 s2 ->
         eval_stmt st s (S_Sequence ast_num c1 c2) s2
 
-with storeUpdate: stack -> name -> value -> Return stack -> Prop := 
-    | SU_Identifier: forall s x v s1 ast_num,
+with storeUpdate: symboltable -> stack -> name -> value -> Return stack -> Prop := 
+    | SU_Identifier: forall s x v s1 st ast_num,
         updateG s x v = Some s1 ->
-        storeUpdate s (E_Identifier ast_num x) v (Normal s1)
-    | SU_Indexed_Component_RTE_E: forall x s a e msg ast_num x_ast_num v,
+        storeUpdate st s (E_Identifier ast_num x) v (Normal s1)
+    | SU_Indexed_Component_RTE_E: forall x s a st e msg ast_num x_ast_num v,
+        fetchG x s = Some a -> (* "a" maybe Undefined or array value *)
+        eval_expr st s e (Run_Time_Error msg) ->
+        storeUpdate st s (E_Indexed_Component ast_num x_ast_num x e) v (Run_Time_Error msg)
+    | SU_Indexed_Component_SubtypeMark_RTE: forall x s a st e i x_ast_num tn a_ast_num tm typ tn' t l u ast_num v,
+        fetchG x s = Some a ->
+        eval_expr st s e (Normal (BasicV (Int i))) ->
+        fetch_exp_type x_ast_num st = Some (Array_Type tn) ->
+        fetch_type tn st = Some (Array_Type_Declaration_SubtypeMark a_ast_num tn tm typ) ->
+        subtype_num tm = Some tn' ->
+        fetch_type tn' st = Some t ->
+        subtype_range t = Some (Range l u) ->
+        do_range_check i l u (Exception RTE_Range) ->
+        storeUpdate st s (E_Indexed_Component ast_num x_ast_num x e) v (Run_Time_Error RTE_Range)
+    | SU_Indexed_Component_Range_RTE: forall x s a st e i x_ast_num t a_ast_num l u typ ast_num v, 
+        fetchG x s = Some a ->
+        eval_expr st s e (Normal (BasicV (Int i))) ->
+        fetch_exp_type x_ast_num st = Some (Array_Type t) ->
+        fetch_type t st = Some (Array_Type_Declaration_Range a_ast_num t (Range l u) typ) ->
+        do_range_check i l u (Exception RTE_Range) ->
+        storeUpdate st s (E_Indexed_Component ast_num x_ast_num x e) v (Run_Time_Error RTE_Range)
+    | SU_Indexed_Component_SubtypeMark_Undef: forall x s st e i x_ast_num tn a_ast_num tm typ tn' t l u v s1 ast_num,
+        fetchG x s = Some Undefined ->
+        eval_expr st s e (Normal (BasicV (Int i))) ->
+        fetch_exp_type x_ast_num st = Some (Array_Type tn) ->
+        fetch_type tn st = Some (Array_Type_Declaration_SubtypeMark a_ast_num tn tm typ) ->
+        subtype_num tm = Some tn' ->
+        fetch_type tn' st = Some t ->
+        subtype_range t = Some (Range l u) ->
+        do_range_check i l u Success ->
+        updateG s x (AggregateV (ArrayV ((i, v) :: nil))) = Some s1 ->
+        storeUpdate st s (E_Indexed_Component ast_num x_ast_num x e) (BasicV v) (Normal s1)
+    | SU_Indexed_Component_SubtypeMark: forall x s a st e i x_ast_num tn a_ast_num tm typ tn' t l u v a1 s1 ast_num,
         fetchG x s = Some (AggregateV (ArrayV a)) ->
-        eval_expr s e (Run_Time_Error msg) ->
-        storeUpdate s (E_Indexed_Component ast_num x_ast_num x e) v (Run_Time_Error msg)
-    | SU_Indexed_Component_RTE_Index: forall x s l u a e i ast_num x_ast_num v,
-        fetchG x s = Some (AggregateV (ArrayV (l, u, a))) ->
-        eval_expr s e (Normal (BasicV (Int i))) ->
-        do_index_check i l u (Exception RTE_Index) ->
-        storeUpdate s (E_Indexed_Component ast_num x_ast_num x e) v (Run_Time_Error RTE_Index)
-    | SU_Indexed_Component: forall x s l u a e i v a1 s1 ast_num x_ast_num,
-        fetchG x s = Some (AggregateV (ArrayV (l, u, a))) ->
-        eval_expr s e (Normal (BasicV (Int i))) ->
-        do_index_check i l u Success ->
+        eval_expr st s e (Normal (BasicV (Int i))) ->
+        fetch_exp_type x_ast_num st = Some (Array_Type tn) ->
+        fetch_type tn st = Some (Array_Type_Declaration_SubtypeMark a_ast_num tn tm typ) ->
+        subtype_num tm = Some tn' ->
+        fetch_type tn' st = Some t ->
+        subtype_range t = Some (Range l u) ->
+        do_range_check i l u Success ->
         arrayUpdate a i v = a1 -> (* a[i] := v *)
-        updateG s x (AggregateV (ArrayV (l, u, a1))) = Some s1 ->
-        storeUpdate s (E_Indexed_Component ast_num x_ast_num x e) (BasicV v) (Normal s1)
-    | SU_Selected_Component: forall r s r1 f v r2 s1 ast_num r_ast_num,
+        updateG s x (AggregateV (ArrayV a1)) = Some s1 ->
+        storeUpdate st s (E_Indexed_Component ast_num x_ast_num x e) (BasicV v) (Normal s1)
+    | SU_Indexed_Component_Range_Undef: forall x s st e i x_ast_num t a_ast_num l u typ s1 ast_num v, 
+        fetchG x s = Some Undefined ->
+        eval_expr st s e (Normal (BasicV (Int i))) ->
+        fetch_exp_type x_ast_num st = Some (Array_Type t) ->
+        fetch_type t st = Some (Array_Type_Declaration_Range a_ast_num t (Range l u) typ) ->
+        do_range_check i l u Success ->
+        updateG s x (AggregateV (ArrayV ((i, v) :: nil))) = Some s1 ->
+        storeUpdate st s (E_Indexed_Component ast_num x_ast_num x e) (BasicV v) (Run_Time_Error RTE_Range)
+    | SU_Indexed_Component_Range: forall x s a st e i x_ast_num t a_ast_num l u typ a1 s1 ast_num v, 
+        fetchG x s = Some (AggregateV (ArrayV a)) ->
+        eval_expr st s e (Normal (BasicV (Int i))) ->
+        fetch_exp_type x_ast_num st = Some (Array_Type t) ->
+        fetch_type t st = Some (Array_Type_Declaration_Range a_ast_num t (Range l u) typ) ->
+        do_range_check i l u Success ->
+        arrayUpdate a i v = a1 -> (* a[i] := v *)
+        updateG s x (AggregateV (ArrayV a1)) = Some s1 ->
+        storeUpdate st s (E_Indexed_Component ast_num x_ast_num x e) (BasicV v) (Normal s1)
+    | SU_Selected_Component_Undef: forall r s f v s1 st ast_num r_ast_num,
+        fetchG r s = Some Undefined ->
+        updateG s r (AggregateV (RecordV ((f, v) :: nil))) = Some s1 -> (* r1.f := v *)
+        storeUpdate st s (E_Selected_Component ast_num r_ast_num r f) (BasicV v) (Normal s1)
+    | SU_Selected_Component: forall r s r1 f v r2 s1 st ast_num r_ast_num,
         fetchG r s = Some (AggregateV (RecordV r1)) ->
         recordUpdate r1 f v = r2 -> (* r1.f := v *)
         updateG s r (AggregateV (RecordV r2)) = Some s1 ->
-        storeUpdate s (E_Selected_Component ast_num r_ast_num r f) (BasicV v) (Normal s1).
+        storeUpdate st s (E_Selected_Component ast_num r_ast_num r f) (BasicV v) (Normal s1).
 
 
 (**********************************************************************************************************
